src/tls/ParsersAux.Binders.Aux.fst
@@ -40,6 +40,43 @@ let serialize_list_clientHelloExtension_eq
   LP.serialize_list_append _ CHE.clientHelloExtension_serializer (L.init l) [L.last l];
   LP.serialize_list_singleton _ CHE.clientHelloExtension_serializer (L.last l)
 
+#push-options "--z3rlimit 16"
+
+let rec serialize_list_eq_parser_fail
+  (#k: LP.parser_kind)
+  (#t: Type)
+  (#p: LP.parser k t)
+  (s: LP.serializer p { k.LP.parser_kind_subkind == Some LP.ParserStrong /\ k.LP.parser_kind_low > 0 })
+  (l1 l2: list t)
+  (b1 b2: LP.bytes)
+: Lemma
+  (requires (
+    LP.serialize (LP.serialize_list _ s) l1 `Seq.append` b1 == LP.serialize (LP.serialize_list _ s) l2 `Seq.append` b2 /\
+    LP.parse p b1 == None /\
+    LP.parse p b2 == None
+  ))
+  (ensures (l1 == l2 /\ b1 == b2))
+  (decreases (L.length l1))
+= LP.serialize_list_nil _ s;
+  assert (b1 `Seq.equal` (Seq.append Seq.empty b1));
+  assert (b2 `Seq.equal` (Seq.append Seq.empty b2));
+  if L.length l2 < L.length l1
+  then serialize_list_eq_parser_fail s l2 l1 b2 b1
+  else match l1, l2 with
+  | [], [] -> ()
+  | x1 :: l1', x2 :: l2' ->
+    LP.serialize_list_cons _ s x1 l1' ;
+    LP.serialize_list_cons _ s x2 l2' ;
+    Seq.append_assoc (LP.serialize s x1) (LP.serialize (LP.serialize_list _ s) l1') b1;
+    Seq.append_assoc (LP.serialize s x2) (LP.serialize (LP.serialize_list _ s) l2') b2;
+    LP.serialize_strong_prefix s x1 x2 (LP.serialize (LP.serialize_list _ s) l1' `Seq.append` b1) (LP.serialize (LP.serialize_list _ s) l2' `Seq.append` b2);
+    serialize_list_eq_parser_fail s l1' l2' b1 b2
+  | [], x2 :: l2' ->
+    LP.serialize_list_cons _ s x2 l2' ;
+    LP.parse_strong_prefix p (LP.serialize s x2) b1
+
+#pop-options
+
 let size32_list_clientHelloExtension
   l
 = LS.size32_list CHE.clientHelloExtension_size32 () l
